C4_diameter_2.v
@@ -12,13 +12,13 @@ Context `{graph_G : Basic_Graph G, pebb_G : Pebbling_Graph G}.
 Notation V := (V G).
 Notation E := (E G).
 
-Hypothesis diam2 : ∀ u v, u = v ∨ E u v ∨ ∃ w, E u w ∧ E w v.
-Hypothesis weight2 : ∀ u v, weight G u v = 2.
 Hypothesis undirected : Symmetric E.
+Hypothesis weight2 : ∀ u v, weight G u v = 2.
+Hypothesis diameter2 : ∀ u v, u = v ∨ E u v ∨ ∃ w, E u w ∧ E w v.
 
-Ltac edge_neq u v :=
+Ltac edge_ne u v :=
   match goal with
-  | H : E u v |- _ => apply irrefl_neq in H as ?
+  | H : E u v |- _ => apply irrefl_ne in H as ?
   end.
 
 Ltac move_pebble s t := eapply rtc_l;
@@ -26,19 +26,38 @@ Ltac move_pebble s t := eapply rtc_l;
   cbn; rewrite ?weight2; [done|try (lia || simpl_alter; clia)|done]|].
 
 Lemma list_choice {X Y} (P : X -> Y -> Prop) xs :
-  (∀ x, x ∈ xs -> ∃ y, P x y) -> ∃ ys, Forall2 P xs ys.
+  Forall (λ x, ∃ y, P x y) xs -> ∃ ys, Forall2 P xs ys.
 Proof.
-Admitted.
+induction xs; inversion_clear 1; [exists []; done|].
+destruct H0 as [y ?]; apply IHxs in H1 as [ys ?].
+exists (y :: ys); constructor; done.
+Qed.
 
 Lemma unnest_fallback {X} (P : X -> Prop) Q (xs : list X) :
   (∀ x, x ∈ xs -> P x ∨ Q) -> (∀ x, x ∈ xs -> P x) ∨ Q.
 Proof.
-Admitted.
+induction xs as [|x xs]; intros H; [left; set_solver|].
+assert (Hx : x ∈ x :: xs) by set_solver; apply H in Hx as []; [|right; done].
+destruct IHxs; [set_solver|left; set_solver|right; done].
+Qed.
 
-Lemma NoDup_dec_witness {X} (xs : list X) :
+Lemma NoDup_dec_witness `{dec : EqDecision X} (xs : list X) :
   NoDup xs + {∃ i j x, i ≠ j ∧ xs !! i = Some x ∧ xs !! j = Some x}.
 Proof.
-Admitted.
+induction xs as [|x xs]; [left; constructor|]; destruct IHxs as [IH|IH].
+- dec (x ∈ xs); [right|left; constructor; done].
+  apply elem_of_list_lookup_1 in H as [i Hi]; exists 0, (S i), x; done.
+- right; destruct IH as (i & j & x' & ? & ? & ?); exists (S i), (S j), x'; cbn.
+  repeat split; [lia|done|done].
+Qed.
+
+Lemma Forall2_elem_of_l {X Y} (P : X -> Y -> Prop) xs ys x :
+  Forall2 P xs ys -> x ∈ xs -> ∃ y, y ∈ ys ∧ P x y.
+Proof.
+intros HP Hx; apply elem_of_list_lookup_1 in Hx as [i Hi].
+eapply Forall2_lookup_l in Hi as (y & Hy & Hxy); [exists y|done].
+split; [apply elem_of_list_lookup_2 in Hy|]; done.
+Qed.
 
 Lemma Forall2_elem_of_r {X Y} (P : X -> Y -> Prop) xs ys y :
   Forall2 P xs ys -> y ∈ ys -> ∃ x, x ∈ xs ∧ P x y.
@@ -50,7 +69,7 @@ Qed.
 
 Notation vs := (enum V).
 
-Theorem pebbling_diameter_2 :
+Theorem pebbling_bound_diameter_2 :
   pebbling_bound G (card V + 1).
 Proof.
 intros t c H; unfold card in H.
@@ -82,16 +101,16 @@ destruct (decide (c t = 0)) as [Ht|?]; [|eexists; split; [done|lia]].
 assert (Hxs : ∀ x, x ∈ xs -> (∃ y, E x y ∧ E y t) ∨ solvable G t 1 c).
 { unfold xs; intros x Hx; apply elem_of_list_filter in Hx as [Hx _].
   assert (x ≠ t) by (intro; subst; lia).
-  destruct (diam2 x t) as [|[]]; [done|right|left; done].
+  destruct (diameter2 x t) as [|[]]; [done|right|left; done].
   eexists; split; [move_pebble x t; done|simpl_alter; lia]. }
 apply unnest_fallback in Hxs as [Hxs|]; [|done].
-apply list_choice in Hxs as [ys ys_spec].
+apply list.Forall_forall, list_choice in Hxs as [ys ys_spec].
 (* Determine ∀ y, y ∈ ys -> c y = 0. *)
 assert (ys_zero : ∀ y, y ∈ ys -> c y = 0 ∨ solvable G t 1 c).
 { intros y Hy; dec (c y = 0); [left; done|right].
   eapply Forall2_elem_of_r in Hy as (x & Hx & Hxy); [|done]; destruct Hxy.
   eapply elem_of_list_filter in Hx as [Hx _].
-  edge_neq x y; edge_neq y t; eexists; split.
+  edge_ne x y; edge_ne y t; eexists; split.
   move_pebble x y; move_pebble y t; done.
   simpl_alter; [|intro; subst]; lia. }
 apply unnest_fallback in ys_zero as [ys_zero|]; [|done].
@@ -104,7 +123,7 @@ destruct (NoDup_dec_witness ys) as [ys_nodup|(i & j & y & ? & Hi & Hj)]. 2:
   eapply Forall2_lookup_r in Hj as (x2 & Hj & Hx); [|done]; destruct Hx;
   assert (x1 ≠ x2) by (intro; subst; eapply NoDup_lookup in xs_nodup; done);
   apply elem_of_list_lookup_2 in Hi, Hj;
-  edge_neq x1 y; edge_neq x2 y; edge_neq y t.
+  edge_ne x1 y; edge_ne x2 y; edge_ne y t.
   eapply elem_of_list_filter in Hi as [Hx1 _], Hj as [Hx2 _].
   eexists; split. move_pebble x1 y; move_pebble x2 y; move_pebble y t; done.
   simpl_alter; [lia|intro|intro]; subst; lia. }
@@ -113,7 +132,7 @@ assert (length0 : t :: ys ⊆+ vs0).
 { apply NoDup_submseteq.
   - apply list.NoDup_cons; split; [|done]; intros Hys.
     eapply Forall2_elem_of_r in Hys as (x & Hx & Hxt); [|done];
-    destruct Hxt; edge_neq t t; done.
+    destruct Hxt; edge_ne t t; done.
   - intros v Hv; apply elem_of_cons in Hv as []; subst;
     apply elem_of_list_filter; split; try apply elem_of_enum; auto. }
 apply submseteq_length in length0; cbn in length0.
@@ -128,7 +147,7 @@ apply elem_of_Permutation in Hvxs as [xs' Hxs].
 assert (Hvxs : v ∈ xs) by (rewrite Hxs; set_solver).
 apply elem_of_list_lookup_1 in Hvxs as [i Hi].
 eapply Forall2_lookup_l in Hi as (y & Hy & HE); [|done]; destruct HE.
-apply elem_of_list_lookup_2 in Hy; clear i; edge_neq v y; edge_neq y t;
+apply elem_of_list_lookup_2 in Hy; clear i; edge_ne v y; edge_ne y t;
 assert (v ≠ t) by (intro; subst; lia).
 rewrite Hxs in xs_nodup; inversion_clear xs_nodup as [|? ? ? xs'_nodup].
 (* Determine zs with Forall2 (λ x z, z ≠ t ∧ E x z ∧ E z v) xs' zs. *)
@@ -136,15 +155,15 @@ assert (Hxs' : ∀ x, x ∈ xs' -> (∃ z, z ≠ t ∧ E x z ∧ E z v) ∨ solv
 { intros x ?; assert (Hx : x ∈ xs) by (rewrite Hxs; set_solver).
   apply elem_of_list_filter in Hx as Hcx; destruct Hcx as [Hcx _].
   assert (x ≠ v) by congruence.
-  destruct (diam2 x v) as [|[|(z & ? & ?)]]; [done|right|].
+  destruct (diameter2 x v) as [|[|(z & ? & ?)]]; [done|right|].
   - dec (y = x); [apply ys_zero in Hy; lia|].
     eexists; split. move_pebble x v; move_pebble v y; move_pebble v y;
     move_pebble y t; done. simpl_alter; [|intro; subst]; lia.
   - dec (z = t); [right|left].
-    + eexists; split; [edge_neq t v; move_pebble v t; done|simpl_alter; lia].
+    + eexists; split; [edge_ne t v; move_pebble v t; done|simpl_alter; lia].
     + exists z; done. }
 apply unnest_fallback in Hxs' as [Hxs'|]; [|done].
-apply list_choice in Hxs' as [zs zs_spec].
+apply list.Forall_forall, list_choice in Hxs' as [zs zs_spec].
 (* Determine ∀ z, z ∈ zs → z ∉ ys. *)
 assert (zs_ys : ∀ z, z ∈ zs -> z ∉ ys ∨ solvable G t 1 c).
 { intros z Hz; destruct (decide (z ∈ ys)) as [Hys|Hys]; [right|left; done].
@@ -153,7 +172,7 @@ assert (zs_ys : ∀ z, z ∈ zs -> z ∉ ys ∨ solvable G t 1 c).
   assert (Hx : x ∈ xs) by (rewrite Hxs; set_solver);
   assert (x ≠ v) by (intro; congruence).
   apply elem_of_list_filter in Hx as [Hx _].
-  edge_neq x z; edge_neq z v; eexists; split.
+  edge_ne x z; edge_ne z v; eexists; split.
   move_pebble v z; move_pebble x z; move_pebble z t; done.
   simpl_alter; [|intro; subst]; lia. }
 apply unnest_fallback in zs_ys as [zs_ys|]; [|done].
@@ -166,7 +185,7 @@ assert (zs_zero : ∀ z, z ∈ zs -> c z = 0 ∨ solvable G t 1 c).
   assert (x ≠ y) by (apply xs_ys; done);
   assert (x ≠ v) by congruence;
   eapply elem_of_list_filter in Hx as [Hx _].
-  edge_neq x z; edge_neq z v; eexists; split.
+  edge_ne x z; edge_ne z v; eexists; split.
   move_pebble x z; move_pebble z v;
   move_pebble v y; move_pebble v y; move_pebble y t; done.
   simpl_alter. lia. intro; subst; lia. }
@@ -186,7 +205,7 @@ destruct (NoDup_dec_witness zs) as [zs_nodup|(i & j & z & ? & Hi & Hj)]. 2:
   assert (x1 ≠ y) by (apply xs_ys; done);
   assert (x2 ≠ y) by (apply xs_ys; done).
   apply elem_of_list_filter in Hx1 as [Hx1 _], Hx2 as [Hx2 _].
-  edge_neq x1 z; edge_neq x2 z; edge_neq z v; eexists; split.
+  edge_ne x1 z; edge_ne x2 z; edge_ne z v; eexists; split.
   move_pebble x1 z; move_pebble x2 z; move_pebble z v;
   move_pebble v y; move_pebble v y; move_pebble y t; done.
   simpl_alter; [|intro|intro]; subst; lia. }
@@ -197,13 +216,26 @@ assert (length0 : t :: zs ++ ys ⊆+ vs0).
     intros Hxy; apply elem_of_app in Hxy as [Hxy|Hxy];
     apply elem_of_list_lookup_1 in Hxy as [i Hi];
     eapply Forall2_lookup_r in Hi as (x & Hi & Hx); [idtac|done|idtac|done];
-    destruct Hx; [|edge_neq t t]; done.
+    destruct Hx; [|edge_ne t t]; done.
   - intros w Hw; apply elem_of_cons in Hw as [Hw|Hw]; subst;
     apply elem_of_list_filter; split; try apply elem_of_enum; try done.
     apply elem_of_app in Hw as []; auto. }
 apply submseteq_length in length0; cbn in length0;
-rewrite app_length in length0.
+erewrite app_length, <-Forall2_length in length0; [|done].
+erewrite <-Forall2_length with (k:=ys) in length0; [|done].
+assert (length xs = length xs' + 1) by (rewrite Hxs; cbn; lia).
+assert (vs0_length : length vs0 ≥ 2 * length xs) by lia.
+revert weight2 H Ht ys_spec vs0_length; clear; intros.
 (* Determine w with c w ≥ 4. *)
-Admitted.
+destruct (decide (Forall (λ k, k ≤ 3) (c <$> xs))) as [Hxs|Hxs].
+apply summation_forall_le in Hxs; rewrite fmap_length in Hxs; lia.
+apply not_Forall_Exists in Hxs; [|solve_decision].
+apply list.Exists_exists in Hxs as (k & Hk & Hw); cbn in Hw.
+apply elem_of_list_fmap in Hk as (w & -> & Hwxs).
+eapply Forall2_elem_of_l in Hwxs as (y & _ & Hy); [|done]; destruct Hy.
+edge_ne w y; edge_ne y t; eexists; split.
+move_pebble w y; move_pebble w y; move_pebble y t; done.
+simpl_alter; [|intro|intro]; subst; lia.
+Qed.
 
 End Diameter_2.
